fstar/test/MLS.Test.Utils.fst
@@ -120,11 +120,11 @@ let uint16_to_ciphersuite x =
   | None -> failwith "couldn't parse ciphersuite"
   | Some cs_nt -> available_ciphersuite_from_network cs_nt
 
-val gen_group_context: {|bytes_like bytes|} -> available_ciphersuite -> bytes -> nat -> bytes -> bytes -> ML bytes
+val gen_group_context: {|bytes_like bytes|} -> available_ciphersuite -> bytes -> nat -> bytes -> bytes -> ML (group_context_nt bytes)
 let gen_group_context cipher_suite group_id epoch tree_hash confirmed_transcript_hash =
   let cipher_suite = available_ciphersuite_to_network cipher_suite in
   if length group_id < pow2 30 && epoch < (pow2 64) && length tree_hash < pow2 30 && length confirmed_transcript_hash < pow2 30 then (
-    (ps_prefix_to_ps_whole ps_group_context_nt).serialize ({
+    {
       version = PV_mls10;
       cipher_suite;
       group_id;
@@ -132,7 +132,7 @@ let gen_group_context cipher_suite group_id epoch tree_hash confirmed_transcript
       tree_hash;
       confirmed_transcript_hash;
       extensions = [];
-    })
+    }
   ) else (
     failwith "gen_group_context: bad data"
   )
